Update proof scripts for common extra invariamts, add extra invariants for example "Massage chair" and add program  for example "Smart lighting"

su.nsk.iae.rpl/xtend-gen/su/nsk/iae/rpl/generator/RPLGenerator.java
@@ -352,7 +352,7 @@ public class RPLGenerator extends AbstractGenerator {
     _builder.append(this.commonExtraInv);
     _builder.append("_def");
     _builder.newLineIfNotEmpty();
-    _builder.append("by force");
+    _builder.append("by (simp;force)");
     _builder.newLine();
     _builder.newLine();
     return _builder.toString();
