examples/MassageChair/Requirements.thy
@@ -5,53 +5,103 @@ begin
 definition R1 where "R1 s \<equiv> 
 always_part (\<lambda> s1. \<not> (getVarBool s1 v_up' = True \<and> getVarBool s1 v_down' = True)) s"
 
+definition Einv1 where "Einv1 s \<equiv> commonExtraInv s \<and>
+always_inv_part (\<lambda> s1. \<not> (getVarBool s1 v_up' = True \<and> getVarBool s1 v_down' = True)) s"
+
 definition R2 where "R2 s \<equiv>
 always_part
-   (\<lambda> s1. getVarBool s1 v_buttonDown' = False \<or> getVarBool s1 v_upper' = True \<longrightarrow> getVarBool s1 v_down' = False) s"
+   (\<lambda> s1. getVarBool s1 v_buttonDown' = False \<or> getVarBool s1 v_lower' = True \<longrightarrow> getVarBool s1 v_down' = False) s"
 
-definition R3 where "R3 s \<equiv> toEnvP s \<and>
-(\<forall> s1. substate s1 s \<and> toEnvP s1 \<and> getVarBool s1 enabled' = False \<longrightarrow>  getVarBool s1 down' = False)"
+definition Einv2 where "Einv2 s \<equiv> commonExtraInv s \<and>
+always_inv_part
+   (\<lambda> s1. getVarBool s1 v_buttonDown' = False \<or> getVarBool s1 v_lower' = True \<longrightarrow> getVarBool s1 v_down' = False) s"
 
-definition R4 where "R4 s \<equiv> toEnvP s \<and>
-(\<forall> s2 s1. substate s1 s2 \<and> substate s2 s \<and> toEnvP s1 \<and> toEnvP s2 \<and> toEnvNum s1 s2 = 1 \<and> getVarBool s1 enabled' = False \<and> getVarBool s2 enabled' = True \<and>
-getVarBool s2 rollerButton' = False \<longrightarrow> getVarBool s2 roller' = False)"
+definition R3 where "R3 s \<equiv> 
+always_part (\<lambda> s1. getVarBool s1 v_enabled' = False \<longrightarrow> getVarBool s1 v_down' = False) s"
 
-definition R5 where "R5 s \<equiv> toEnvP s \<and>
-(\<forall> s1. substate s1 s \<and> toEnvP s1 \<and> getVarBool s1 rollerButton' = PRESSED' \<and> getVarBool s1 enabled' = True \<longrightarrow> getVarBool s1 roller' = True)"
+definition Einv3 where "Einv3 s \<equiv> commonExtraInv s \<and>
+always_inv_part (\<lambda> s1. getVarBool s1 v_enabled' = False \<longrightarrow> getVarBool s1 v_down' = False) s"
 
-abbreviation MASSAGE_TIME where "MASSAGE_TIME \<equiv> ROLLER_MASSAGE_TIME'TIMEOUT + VIBRATION_MASSAGE_TIME'TIMEOUT"
+definition R4 where "R4 s \<equiv> 
+always2_part (\<lambda> s1. getVarBool s1 v_enabled' = False)
+   (\<lambda> s2. getVarBool s2 v_enabled' = True \<and> getVarBool s2 v_rollerButton' = False)
+   (\<lambda> s2. getVarBool s2 v_roller' = False) s"
 
-definition R6 where "R6 s \<equiv> toEnvP s \<and>
-P1 s MASSAGE_TIME (\<lambda> s1. getVarBool s1 roller' = True \<or> getVarBool s1 vibration' = True)
- (\<lambda> s3. getVarBool s3 roller' = False \<and> getVarBool s3 vibration' = False \<or> getVarBool s3 startButton' = PRESSED')
-(\<lambda> s2. (getVarBool s2 roller' = True \<or> getVarBool s2 vibration' = True) \<and> getVarBool s2 startButton' \<noteq> PRESSED')"
+definition Einv4 where "Einv4 s \<equiv> commonExtraInv s \<and>
+always2_inv_part (\<lambda> s. getPstate s p_Controller' \<in> {p_Controller's_turnedOn', p_Controller's_turningOff'})
+   (\<lambda> s1. getVarBool s1 v_enabled' = False)
+   (\<lambda> s2. getVarBool s2 v_enabled' = True \<and> getVarBool s2 v_rollerButton' = False)
+   (\<lambda> s2. getVarBool s2 v_roller' = False) s"
 
-definition R7 where "R7 s \<equiv> toEnvP s \<and>
-(\<forall> s1 s2. substate s1 s2 \<and> substate s2 s \<and> toEnvP s1 \<and> toEnvP s2 \<and> toEnvNum s1 s2 > ON_OFF_TIME'TIMEOUT  \<and> (getVarBool s1 enabled' = True) \<and>
- (getVarBool s2 onOff' \<noteq> PRESSED') \<and>
-(\<forall>  s3. toEnvP s3 \<and>substate s1 s3 \<and> substate s3 s2 \<and> s1 \<noteq> s3 \<and> s3 \<noteq> s2 \<longrightarrow> getVarBool s3 onOff' = PRESSED') \<longrightarrow>
-getVarBool s2 roller' = False \<and> getVarBool s2 vibration' = False)"
+definition R5 where "R5 s \<equiv> 
+always_part (\<lambda> s1. getVarBool s1 v_rollerButton' = v_PRESSED' \<and> getVarBool s1 v_enabled' = True \<longrightarrow>
+   getVarBool s1 v_roller' = True) s"
 
-definition R7_1 where "R7_1 s \<equiv> toEnvP s \<and>
-P2 s (\<lambda> s1 s2.  P12op s1 ON_OFF_TIME'TIMEOUT (\<lambda> s3. getVarBool s3 enabled' = True)  (\<lambda> s4. getVarBool s4 onOff' = PRESSED') \<and> getVarBool s2 onOff' \<noteq> PRESSED')
- (\<lambda> s1 s2. getVarBool s2 roller' = False \<and> getVarBool s2 vibration' = False)
-"
+definition Einv5 where "Einv5 s \<equiv> commonExtraInv s \<and>
+always_inv_part (\<lambda> s1. getVarBool s1 v_rollerButton' = v_PRESSED' \<and> getVarBool s1 v_enabled' = True \<longrightarrow>
+   getVarBool s1 v_roller' = True) s"
 
-definition R8 where "R8 s \<equiv> toEnvP s \<and>
-(\<forall> s1 s2 s4. substate s1 s2 \<and> substate s2 s4 \<and> substate s4 s \<and> toEnvP s1 \<and> toEnvP s2 \<and> toEnvP s4 \<and> toEnvNum s1 s2 > ON_OFF_TIME'TIMEOUT  \<and> (getVarBool s1 enabled' = True) \<and>
- (getVarBool s2 onOff' \<noteq> PRESSED') \<and>
-(\<forall>  s3. toEnvP s3 \<and>substate s1 s3 \<and> substate s3 s2 \<and> s1 \<noteq> s3 \<and> s3 \<noteq> s2 \<longrightarrow> getVarBool s3 onOff' = PRESSED') \<and>
-(\<forall> s5. toEnvP s5 \<and> substate s2 s5 \<and> substate s5 s4 \<longrightarrow> getVarBool s5 upper' = False) \<longrightarrow>
-getVarBool s4 up' = True)"
+abbreviation MASSAGE_TIME where "MASSAGE_TIME \<equiv> v_ROLLER_MASSAGE_TIME'TIMEOUT + v_VIBRATION_MASSAGE_TIME'TIMEOUT"
 
+definition R6 where "R6 s \<equiv> 
+P1_1_part MASSAGE_TIME (\<lambda> s1. getVarBool s1 v_roller' = True \<or> getVarBool s1 v_vibration' = True)
+(\<lambda> s2. (getVarBool s2 v_roller' = True \<or> getVarBool s2 v_vibration' = True) \<and> getVarBool s2 v_startButton' \<noteq> v_PRESSED')
+ (\<lambda> s3. getVarBool s3 v_roller' = False \<and> getVarBool s3 v_vibration' = False \<or> getVarBool s3 v_startButton' =
+   v_PRESSED')
+  s"
 
-definition R8_1 where "R8_1 s \<equiv> toEnvP s \<and>
-P6 s (\<lambda> s3 s4. P12op s3 ON_OFF_TIME'TIMEOUT (\<lambda> s1. getVarBool s1 enabled' = True) (\<lambda> s2. getVarBool s2 onOff' = PRESSED') \<and> getVarBool s4 onOff' \<noteq> PRESSED')
-(\<lambda> s5. getVarBool s5 up' = True) (\<lambda> s6. getVarBool s6 upper' = True)"
+definition Einv6 where "Einv6 s \<equiv> commonExtraInv s \<and>
+P1_1_inv_part MASSAGE_TIME
+   (\<lambda> s.
+    if getPstate s p_Roller' \<noteq> p_Roller's_massaging' \<and> getPstate s p_Vibration' \<noteq> p_Vibration's_massaging' then 0 
+    else if getPstate s p_Roller' = p_Roller's_waiting' \<and> getPstate s p_Vibration' = p_Vibration's_massaging'
+      then ltime s p_Vibration'
+    else if getPstate s p_Roller' = p_Roller's_massaging' \<and> getPstate s p_Vibration' = p_Vibration's_waiting'
+      then ltime s p_Roller'
+    else if getPstate s p_Roller' = STOP \<and> getPstate s p_Vibration' = p_Vibration's_massaging' 
+      then (v_ROLLER_MASSAGE_TIME'TIMEOUT + ltime s p_Vibration')
+    else if getPstate s p_Roller' = p_Roller's_massaging' \<and> getPstate s p_Vibration' = STOP
+      then (v_VIBRATION_MASSAGE_TIME'TIMEOUT + ltime s p_Roller')
+    else if getPstate s p_Roller' = p_Roller's_massaging' \<and> getPstate s p_Vibration' = p_Vibration's_massaging' \<and>
+      ltime s p_Roller' \<le> ltime s p_Vibration'
+      then ltime s p_Vibration'
+    else ltime s p_Roller')
+   (\<lambda> s1. getVarBool s1 v_roller' = True \<or> getVarBool s1 v_vibration' = True)
+(\<lambda> s2. (getVarBool s2 v_roller' = True \<or> getVarBool s2 v_vibration' = True) \<and> getVarBool s2 v_startButton' \<noteq> v_PRESSED')
+ (\<lambda> s3. getVarBool s3 v_roller' = False \<and> getVarBool s3 v_vibration' = False \<or> getVarBool s3 v_startButton' =
+   v_PRESSED')
+  s"
 
+definition R7 where "R7 s \<equiv> 
+P6_1_part v_ON_OFF_TIME'TIMEOUT (\<lambda> s1. getVarBool s1 v_enabled' = True)
+   (\<lambda> s2. getVarBool s2 v_onOff' = v_PRESSED') (\<lambda> s3. getVarBool s3 v_onOff' \<noteq> v_PRESSED')
+    (\<lambda> s3. getVarBool s3 v_roller' = False \<and> getVarBool s3 v_vibration' = False) s"
 
-definition R9 where "R9 s \<equiv> toEnvP s \<and>
-P6 s (\<lambda> s1 s2. getVarBool s1 enabled' = True \<and> getVarBool s2 enabled' = False) (\<lambda> s3. getVarBool s3 up' = True) (\<lambda> s4. getVarBool s4 upper' = True)"
+definition Einv7 where "Einv7 s \<equiv> commonExtraInv s \<and>
+P6_1_inv_part v_ON_OFF_TIME'TIMEOUT
+  (\<lambda> s. getPstate s p_Controller' \<noteq> p_Controller's_turningOff')
+   (\<lambda> s. if getPstate s p_Controller' = p_Controller's_turnedOn' then ltime s p_Controller' else 0)
+  (\<lambda> s. getPstate s p_Controller' \<noteq> p_Controller's_turningOff')
+   (\<lambda> s1. getVarBool s1 v_enabled' = True)
+   (\<lambda> s2. getVarBool s2 v_onOff' = v_PRESSED') (\<lambda> s3. getVarBool s3 v_onOff' \<noteq> v_PRESSED')
+    (\<lambda> s3. getVarBool s3 v_roller' = False \<and> getVarBool s3 v_vibration' = False) s"
+
+definition R8 where "R8 s \<equiv> 
+P6_2_part v_ON_OFF_TIME'TIMEOUT (\<lambda> s1. getVarBool s1 v_enabled' = True)
+   (\<lambda> s2. getVarBool s2 v_onOff' = v_PRESSED') (\<lambda> s3. getVarBool s3 v_onOff' \<noteq> v_PRESSED')
+    (\<lambda> s4. getVarBool s4 v_up' = True) (\<lambda> s5. getVarBool s5 v_upper' = True)
+   s"
+
+definition Einv8 where "Einv8 s \<equiv> commonExtraInv s \<and>
+P6_2_inv_part v_ON_OFF_TIME'TIMEOUT
+  (\<lambda> s. getPstate s p_Controller' \<noteq> p_Controller's_turningOff')
+   (\<lambda> s. if getPstate s p_Controller' = p_Controller's_turnedOn' then ltime s p_Controller' else 0)
+  (\<lambda> s. getPstate s p_Controller' \<noteq> p_Controller's_turningOff')
+  (\<lambda> s. getPstate s p_Controller' = p_Controller's_backLifting' \<and> getVarBool s v_up' = True)
+   (\<lambda> s1. getVarBool s1 v_enabled' = True)
+   (\<lambda> s2. getVarBool s2 v_onOff' = v_PRESSED') (\<lambda> s3. getVarBool s3 v_onOff' \<noteq> v_PRESSED')
+    (\<lambda> s4. getVarBool s4 v_up' = True) (\<lambda> s5. getVarBool s5 v_upper' = True)
+   s"
 
 end
 
