examples/SmartLighting/ExtraInv_R2.thy
@@ -1,0 +1,157 @@
+theory ExtraInv_R2
+  imports CommonExtraInv "../Patterns"
+begin
+
+definition extraInv where "extraInv s \<equiv> commonExtraInv s \<and>
+(getPstate s Motion' = Motion'noMovement' \<longrightarrow>
+P5_1inv s LIGHTING_TIME'TIMEOUT (LIGHTING_TIME'TIMEOUT - 1) (\<lambda> s1.  getVarBool s1 motion' = True \<and>  getVarBool s1 light' = LOW')
+  (\<lambda> s3. P2all s3 (\<lambda> s2. getVarInt s2 timeOfDay' = NIGHT' \<or> getVarInt s3 timeOfDay' = NIGHT' \<or>
+ getVarBool s3 dayLight' = True \<or> getVarBool s3 dimLight' = True))) \<and>
+(getPstate s Motion' = Motion'movement' \<longrightarrow>
+P5_1inv s LIGHTING_TIME'TIMEOUT (ltime s Motion' - 1) (\<lambda> s1.  getVarBool s1 motion' = True \<and>  getVarBool s1 light' = LOW')
+  (\<lambda> s3. P2all s3 (\<lambda> s2. getVarInt s2 timeOfDay' = NIGHT' \<or> getVarInt s3 timeOfDay' = NIGHT' \<or>
+ getVarBool s3 dayLight' = True \<or> getVarBool s3 dimLight' = True)))"
+
+theorem extra1: "VC1 extraInv ss0"
+  apply(unfold VC1_def extraInv_def commonExtraInv_def P5_1inv_rule)
+  apply auto
+  done
+
+theorem extra146: "VC146 extraInv env s0 motion_value light_value"
+  apply(unfold VC146_def extraInv_def)
+  apply(rule impI)
+  apply(rule conjI)
+  using cei146 VC146_def apply auto[1]
+ apply(unfold commonExtraInv_def)
+  apply(erule conjE)+
+  apply(rule conjI)
+  subgoal
+    apply simp
+    done
+  subgoal
+    apply(simp;((rule impI;simp)?);rule P5_1inv_rule[of s0])
+        apply simp
+    subgoal
+      apply simp
+      apply(rule P2all_rule[of s0])
+       apply simp
+      by simp
+      apply simp
+     apply simp
+    by simp
+  done
+
+theorem extra164: "VC164 extraInv env s0 motion_value light_value"
+  apply(unfold VC164_def extraInv_def)
+  apply(rule impI)
+  apply(rule conjI)
+  using cei164 VC164_def apply auto[1]
+ apply(unfold commonExtraInv_def)
+  apply(erule conjE)+
+  apply(rule conjI)
+  subgoal
+    apply(simp;((rule impI;simp)?);rule P5_1inv_rule[of s0])
+        apply simp
+       apply simp
+      apply simp
+     apply simp
+    by simp
+  by simp
+
+theorem extra82: "VC182 extraInv env s0 motion_value light_value"
+  apply(unfold VC182_def extraInv_def)
+  apply(rule impI)
+  apply(rule conjI)
+  using cei182 VC182_def apply auto[1]
+ apply(unfold commonExtraInv_def)
+  apply(erule conjE)+
+  by simp
+
+theorem extra200: "VC200 extraInv env s0 motion_value light_value"
+  apply(unfold VC200_def extraInv_def)
+  apply(rule impI)
+  apply(rule conjI)
+  using cei200 VC200_def apply auto[1]
+ apply(unfold commonExtraInv_def)
+  apply(erule conjE)+
+  apply(rule conjI)
+   apply simp
+  subgoal
+    apply(simp;((rule impI;simp)?);rule P5_1inv_rule[of s0])
+        apply simp
+      apply simp
+      apply(cases light_value)
+        apply simp
+    subgoal
+      apply simp
+      apply(rule P2all_rule[of s0])
+       apply simp
+      by simp
+    subgoal
+      apply simp
+      apply(rule imp_rule)
+        apply assumption
+       apply(rule P2all_rule[of s0])
+      apply simp
+       apply assumption
+      by simp
+     apply simp
+    by simp
+  done
+
+theorem extra218: "VC218 extraInv env s0 motion_value light_value"
+  apply(unfold VC218_def extraInv_def)
+  apply(rule impI)
+  apply(rule conjI)
+  using cei218 VC218_def apply auto[1]
+ apply(unfold commonExtraInv_def)
+  apply(erule conjE)+
+  apply(rule conjI)
+   apply(simp;(rule impI; simp)?)
+   apply(rule P5_1inv_rule[of s0])
+       apply simp
+      apply simp
+     apply simp
+    apply simp
+   apply simp
+  by simp
+
+theorem extra236: "VC236 extraInv env s0 motion_value light_value"
+  apply(unfold VC236_def extraInv_def)
+  apply(rule impI)
+  apply(rule conjI)
+  using cei236 VC236_def apply auto[1]
+ apply(unfold commonExtraInv_def)
+  apply(erule conjE)+
+  apply(rule conjI)
+   apply simp
+  apply(simp;(rule impI; simp)?) 
+  apply(rule P5_1inv_rule[of s0])
+      apply simp
+     apply simp
+    apply simp
+    apply(rule P2all_rule[of s0])
+     apply simp
+    apply simp
+   apply simp
+  by simp
+
+theorem extra254: "VC254 extraInv env s0 motion_value light_value"
+  apply(unfold VC254_def extraInv_def)
+  apply(rule impI)
+  apply(rule conjI)
+  using cei254 VC254_def apply auto[1]
+ apply(unfold commonExtraInv_def)
+  apply(erule conjE)+
+  by simp
+
+theorem extra272: "VC272 extraInv env s0 motion_value light_value"
+  apply(unfold VC272_def extraInv_def)
+  apply(rule impI)
+  apply(rule conjI)
+  using cei272 VC272_def apply auto[1]
+ apply(unfold commonExtraInv_def)
+  apply(erule conjE)+
+  by simp
+
+end
