examples/SmartLighting/ExtraInv_R2_1.thy
@@ -1,0 +1,107 @@
+theory ExtraInv_R2_1
+  imports CommonExtraInv Requirements
+begin
+
+definition extraInv where "extraInv s \<equiv> commonExtraInv s \<and>
+(getPstate s Motion' = Motion'movement' \<longrightarrow>
+P7inv s LIGHTING_TIME'TIMEOUT (ltime s Motion' - 1) (\<lambda> s1 s2. getVarInt s1 timeOfDay' \<noteq> NIGHT' \<and> getVarInt s2 timeOfDay' \<noteq> NIGHT' \<and> getVarBool s2 motion' \<and> getVarBool s2 light' = LOW')
+(\<lambda> s4. getVarInt s4 timeOfDay' = NIGHT') (\<lambda> s3. getVarBool s3 dayLight' = TURNED_ON' \<or> getVarBool s3 dimLight' = TURNED_ON')) \<and>
+(getPstate s Motion' \<noteq> Motion'movement' \<longrightarrow>
+P7inv s LIGHTING_TIME'TIMEOUT (LIGHTING_TIME'TIMEOUT - 1) (\<lambda> s1 s2. getVarInt s1 timeOfDay' \<noteq> NIGHT' \<and> getVarInt s2 timeOfDay' \<noteq> NIGHT' \<and> getVarBool s2 motion' \<and> getVarBool s2 light' = LOW')
+(\<lambda> s4. getVarInt s4 timeOfDay' = NIGHT') (\<lambda> s3. getVarBool s3 dayLight' = TURNED_ON' \<or> getVarBool s3 dimLight' = TURNED_ON'))"
+
+theorem extra1: "VC1 extraInv s0"
+  apply(unfold VC1_def extraInv_def commonExtraInv_def P7inv_def)
+  apply auto
+  done
+
+theorem extra148: "VC148 extraInv env s0 motion_value light_value"
+  apply(unfold VC148_def extraInv_def)
+  apply(rule impI)
+  apply(rule conjI)
+  using cei148 VC148_def apply auto[1]
+ apply(unfold commonExtraInv_def)
+  apply(erule conjE)+
+  apply(rule conjI)
+   apply(simp;(rule impI;simp)?)
+   apply(rule P7inv_rule[of s0])
+       apply auto
+  done
+
+theorem extra166: "VC166 extraInv env s0 motion_value light_value"
+  apply(unfold VC166_def extraInv_def)
+  apply(rule impI)
+  apply(rule conjI)
+  using cei166 VC166_def apply auto[1]
+ apply(unfold commonExtraInv_def)
+  apply(erule conjE)+
+  apply simp
+  done
+
+theorem extra184: "VC184 extraInv env s0 motion_value light_value"
+  apply(unfold VC184_def extraInv_def)
+  apply(rule impI)
+  apply(rule conjI)
+  using cei184 VC184_def apply auto[1]
+ apply(unfold commonExtraInv_def)
+  apply(erule conjE)+
+  apply simp
+  done
+
+theorem extra202: "VC202 extraInv env s0 motion_value light_value"
+  apply(unfold VC202_def extraInv_def)
+  apply(rule impI)
+  apply(rule conjI)
+  using cei202 VC202_def apply auto[1]
+ apply(unfold commonExtraInv_def)
+  apply(erule conjE)+
+  apply(rule conjI)
+   apply(simp;(rule impI;simp)?)
+   apply(rule P7inv_rule[of s0])
+       apply auto
+  done
+
+theorem extra220: "VC220 extraInv env s0 motion_value light_value"
+  apply(unfold VC220_def extraInv_def)
+  apply(rule impI)
+  apply(rule conjI)
+  using cei220 VC220_def apply auto[1]
+ apply(unfold commonExtraInv_def)
+  apply(erule conjE)+
+  apply simp
+  done
+
+theorem extra238: "VC238 extraInv env s0 motion_value light_value"
+  apply(unfold VC238_def extraInv_def)
+  apply(rule impI)
+  apply(rule conjI)
+  using cei238 VC238_def apply auto[1]
+ apply(unfold commonExtraInv_def)
+  apply(erule conjE)+
+  apply(rule conjI)
+   apply(simp;(rule impI;simp)?)
+   apply(rule P7inv_rule[of s0])
+       apply auto
+  done
+
+theorem extra256: "VC256 extraInv env s0 motion_value light_value"
+  apply(unfold VC256_def extraInv_def)
+  apply(rule impI)
+  apply(rule conjI)
+  using cei256 VC256_def apply auto[1]
+ apply(unfold commonExtraInv_def)
+  apply(erule conjE)+
+  apply simp
+  done
+
+theorem extra274: "VC274 extraInv env s0 motion_value light_value"
+  apply(unfold VC274_def extraInv_def)
+  apply(rule impI)
+  apply(rule conjI)
+  using cei274 VC274_def apply auto[1]
+ apply(unfold commonExtraInv_def)
+  apply(erule conjE)+
+  apply simp
+  done
+
+end
