examples/SmartLighting/ExtraInv_R7.thy
@@ -1,0 +1,102 @@
+theory ExtraInv_R7
+  imports CommonExtraInv "../Patterns"
+begin
+
+definition extraInv where "extraInv s \<equiv> commonExtraInv s \<and>
+(getPstate s Motion' = Motion'movement' \<longrightarrow> 
+always s (\<lambda> s1. getVarBool s1 motion' = False \<longrightarrow> constrained_until_inv s1 s (LIGHTING_TIME'TIMEOUT + MORNING_LIGHTING_TIME'TIMEOUT) (ltime s Motion' - 1)
+(\<lambda> s2. (getVarBool s2 dayLight' = True \<or> getVarBool s2 dimLight' = True) \<and> getVarBool s2 motion' = False)
+ (\<lambda> s3. getVarBool s3 dayLight' = False \<and> getVarBool s3 dimLight'= False \<or> getVarBool s3 motion' = True))) \<and>
+(getPstate s Motion' \<noteq>  Motion'movement' \<and> getPstate s Lighting' = Lighting'morningLighting' \<longrightarrow> 
+always s (\<lambda> s1. getVarBool s1 motion' = False \<longrightarrow> constrained_until_inv s1 s (LIGHTING_TIME'TIMEOUT + MORNING_LIGHTING_TIME'TIMEOUT)
+ (LIGHTING_TIME'TIMEOUT + ltime s Lighting' - 1)
+(\<lambda> s2. (getVarBool s2 dayLight' = True \<or> getVarBool s2 dimLight' = True) \<and> getVarBool s2 motion' = False)
+ (\<lambda> s3. getVarBool s3 dayLight' = False \<and> getVarBool s3 dimLight'= False \<or> getVarBool s3 motion' = True))) \<and>
+(getPstate s Motion' \<noteq>  Motion'movement' \<and> getPstate s Lighting' = Lighting'morningOrDay' \<longrightarrow> 
+always s (\<lambda> s1. getVarBool s1 motion' = False \<longrightarrow> constrained_until_inv s1 s (LIGHTING_TIME'TIMEOUT + MORNING_LIGHTING_TIME'TIMEOUT)
+(LIGHTING_TIME'TIMEOUT + MORNING_LIGHTING_TIME'TIMEOUT)
+(\<lambda> s2. (getVarBool s2 dayLight' = True \<or> getVarBool s2 dimLight' = True) \<and> getVarBool s2 motion' = False)
+ (\<lambda> s3. getVarBool s3 dayLight' = False \<and> getVarBool s3 dimLight'= False \<or> getVarBool s3 motion' = True)))  \<and>
+(getPstate s Motion' \<noteq>  Motion'movement' \<and> getPstate s Lighting' \<in> {Lighting'night', Lighting'earlyMorning', Lighting'evening'} \<longrightarrow> 
+always s (\<lambda> s1. getVarBool s1 motion' = False \<longrightarrow> constrained_until_inv s1 s (LIGHTING_TIME'TIMEOUT + MORNING_LIGHTING_TIME'TIMEOUT) 0
+(\<lambda> s2. (getVarBool s2 dayLight' = True \<or> getVarBool s2 dimLight' = True) \<and> getVarBool s2 motion' = False)
+ (\<lambda> s3. getVarBool s3 dayLight' = False \<and> getVarBool s3 dimLight'= False \<or> getVarBool s3 motion' = True)))"
+
+theorem extra1: "VC1 extraInv s0"
+  apply(unfold VC1_def extraInv_def commonExtraInv_def always_def constrained_until_inv_def)
+  apply auto
+  done  
+
+theorem extra148: "VC148 extraInv env s0 motion_value light_value"
+  apply(unfold VC148_def extraInv_def)
+  apply(rule impI)
+  apply(rule conjI)
+  using cei148 VC148_def apply auto[1]
+ apply(unfold commonExtraInv_def)
+  apply(erule conjE)+
+  apply(rule conjI)
+   apply(simp;(rule impI;simp)?)
+  apply(simp only: imp_conv_disj)
+   apply(rule always_rule[of s0])
+    apply(rule conj_forward)
+      prefer 2
+      apply(rotate_tac -1)
+      apply assumption
+     prefer 2
+     apply(rule conj_forward)
+       prefer 2
+       apply(rule disj_forward)
+         prefer 2
+      apply(rotate_tac -1)
+         apply assumption
+        prefer 2
+        apply(rule constrained_until_one_point)
+         apply simp
+      apply(rotate_tac -1)
+        apply assumption
+      apply(rotate_tac -1)
+       apply assumption
+      prefer 2
+      apply(rule all_disj_rule)
+      apply(rule conj_forward)
+        prefer 2
+  apply(rule all_imp_refl)
+      apply(rotate_tac -1)
+        apply assumption
+       prefer 2 
+       apply(rule constrained_until_rule[of s0])
+        apply simp
+       apply(rule conj_forward)
+         prefer 2
+         apply(rule all_imp_refl)
+         apply(rotate_tac -1)
+         apply assumption
+        prefer 2
+        apply(rule conj_forward)
+          prefer 2
+        apply(rule all_imp_refl)
+         apply(rotate_tac -1)
+          apply assumption
+         prefer 2
+         apply(rotate_tac -1)
+         apply assumption
+         apply(rotate_tac -1)
+        apply assumption
+         apply(rotate_tac -1)
+       apply assumption
+         apply(rotate_tac -1)
+      apply assumption
+         apply(rotate_tac -1)
+     apply assumption
+    apply auto[2]
+  apply(rule conjI)
+   apply simp
+  apply simp
+  done
+
+
+
+
+
+
+
