examples/SmartLighting/Requirements.thy
@@ -1,0 +1,44 @@
+theory Requirements
+  imports CommonExtraInv VCProving.Basic_Patterns VCProving.Derived_Patterns
+begin
+
+definition R1 where "R1 s \<equiv>
+always_part (\<lambda> s1. getVarInt s1 v_timeOfDay' = v_NIGHT' \<longrightarrow> getVarBool s1 v_dayLight' = False \<and> getVarBool s1 v_dimLight' = False) s"
+
+definition R2 where "R2 s \<equiv> 
+P4_2_part v_LIGHTING_TIME'TIMEOUT (\<lambda> s1. getVarInt s1 v_timeOfDay' \<noteq> v_NIGHT')
+  (\<lambda> s2. getVarInt s2 v_timeOfDay' \<noteq> v_NIGHT' \<and> getVarBool s2 v_motion' = True \<and> getVarBool s v_light' = v_LOW')
+ (\<lambda> s3. getVarBool s3 v_dayLight' = v_TURNED_ON' \<or> getVarBool s3 v_dimLight' = v_TURNED_ON') (\<lambda> s4. getVarInt s4 v_timeOfDay' = v_NIGHT') s"
+
+
+definition R3 where "R3 s ==
+P2_2_part (v_MORNING_LIGHTING_TIME'TIMEOUT + 1) (\<lambda> s1. getVarInt s1 v_timeOfDay' = v_EARLY_MORNING')
+   (\<lambda> s2. getVarInt s2 v_timeOfDay' = v_MORNING_LIGHTING') (\<lambda> s3. getVarBool s3 v_dimLight' = v_TURNED_ON') s"
+
+definition R4 where "R4 s \<equiv> 
+  always2_part (\<lambda> s1. getVarInt s1 v_timeOfDay' = v_DAY') (\<lambda> s2. True) (\<lambda> s2. getVarBool s2 v_dimLight' = False) s"
+
+definition R5 where "R5 s \<equiv> 
+always2_part (\<lambda> s1. getVarInt s1 v_timeOfDay' = v_EVENING') (\<lambda> s2. True) (\<lambda> s2. getVarBool s2 v_dayLight' = False) s"
+
+definition R6 where "R6 s == toEnvP s \<and>
+(\<forall> s1. substate s1 s \<and> toEnvP s1 \<and> getVarBool s1 dayLight' = TURNED_ON' \<longrightarrow> getVarBool s1 dimLight' = TURNED_OFF')"
+
+definition R7 where "R7  s \<equiv> toEnvP s \<and>
+P1 s (LIGHTING_TIME'TIMEOUT + MORNING_LIGHTING_TIME'TIMEOUT) (\<lambda> s1. getVarBool s1 motion' = False)
+ (\<lambda> s3. getVarBool s3 dayLight' = False \<and> getVarBool s3 dimLight'= False \<or> getVarBool s3 motion' = True)
+(\<lambda> s2. (getVarBool s2 dayLight' = True \<or> getVarBool s2 dimLight' = True) \<and> getVarBool s2 motion' = False)"
+
+definition R7_1 where "R7_1 s \<equiv> toEnvP s \<and>
+always s (\<lambda> s1. getVarBool s1 motion' = False \<longrightarrow> constrained_until s1 s (LIGHTING_TIME'TIMEOUT + MORNING_LIGHTING_TIME'TIMEOUT)
+(\<lambda> s2. (getVarBool s2 dayLight' = True \<or> getVarBool s2 dimLight' = True) \<and> getVarBool s2 motion' = False)
+ (\<lambda> s3. getVarBool s3 dayLight' = False \<and> getVarBool s3 dimLight'= False \<or> getVarBool s3 motion' = True))"
+
+definition R8 where "R8 s \<equiv> toEnvP s \<and>
+P1 s (LIGHTING_TIME'TIMEOUT - 1) (\<lambda> s2. P2ex s2 (\<lambda> s1. getVarBool s1 motion' = True \<and> getVarBool s2 motion' = False))
+ (\<lambda> s3. getVarBool s3 dayLight' = False \<and> getVarBool s3 dimLight'= False \<or> getVarBool s3 motion' = True \<or>
+ P2ex s3 (\<lambda> s2'.  getVarInt s2' timeOfDay' = MORNING_LIGHTING' \<or> getVarInt s3 timeOfDay' = MORNING_LIGHTING'))
+(\<lambda> s2. (getVarBool s2 dayLight' = True \<or> getVarBool s2 dimLight' = True) \<and> getVarBool s2 motion' = False \<and>
+ P2all s2 (\<lambda> s1'. getVarInt s1' timeOfDay' \<noteq> MORNING_LIGHTING' \<and>getVarInt s2 timeOfDay' \<noteq> MORNING_LIGHTING'))"
+
+end
